src/cddl/pulse/CDDL.Pulse.Bundle.MapGroup.fst
@@ -1,6 +1,7 @@
 module CDDL.Pulse.Bundle.MapGroup
 include CDDL.Pulse.Bundle.Base
 include CDDL.Pulse.Parse.MapGroup
+include CDDL.Pulse.Serialize.MapGroup
 open Pulse.Lib.Pervasives
 open CBOR.Spec.API.Type
 open CBOR.Pulse.API.Base
@@ -21,16 +22,39 @@ type map_bundle
   mb_impl_type: Type0;
   [@@@erasable] mb_rel: rel mb_impl_type mb_spec_type;
   mb_parser: impl_zero_copy_map_group vmatch mb_spec.mg_parser mb_rel;
+  mb_serializer: impl_serialize_map_group mb_spec mb_rel;
 }
+
+unfold
+let impl_serialize_map_ext_precond
+    (#t1: (det_map_group))
+    (#fp1: typ)
+    (#tgt1: Type0)
+    (#inj1: bool)
+    (ps1: (mg_spec t1 fp1 tgt1 inj1))
+    (#t2: det_map_group)
+    (#fp2: typ)
+    (#inj2: bool)
+    (ps2: (mg_spec t2 fp2 tgt1 inj2))
+: Tot prop
+=
+      t2 == t1 /\
+      (forall (x: tgt1) . (ps2).mg_serializable x <==> (ps1).mg_serializable x) /\
+      (forall (x: tgt1) . (ps2).mg_serializable x ==> (
+        (ps1).mg_serializable x /\
+        (ps2).mg_serializer x `cbor_map_equal` (ps1).mg_serializer x
+      )) /\
+      (forall (x: tgt1) . (ps2).mg_size x == (ps1).mg_size x)
 
 inline_for_extraction noextract [@@noextract_to "krml"; bundle_get_impl_type_attr ]
 let bundle_map
   (#ty: Type0)
   (#vmatch: perm -> ty -> cbor -> slprop)
+  (cbor_serialize_map: cbor_det_serialize_map_t)
   (mb: map_bundle vmatch)
 : Tot (bundle vmatch)
 = match mb with
-  | Mkmap_bundle mb_typ mb_footprint mb_footprint_correct mb_spec_type mb_spec_type_eq mb_spec mb_impl_type mb_rel mb_parser ->
+  | Mkmap_bundle mb_typ mb_footprint mb_footprint_correct mb_spec_type mb_spec_type_eq mb_spec mb_impl_type mb_rel mb_parser mb_serializer ->
 {
   b_typ = _;
   b_spec_type = _;
@@ -39,6 +63,7 @@ let bundle_map
   b_impl_type = _;
   b_rel = _;
   b_parser = impl_zero_copy_map mb_parser ();
+  b_serializer = impl_serialize_map cbor_serialize_map mb_serializer ();
 }
 
 inline_for_extraction noextract [@@noextract_to "krml"; bundle_get_impl_type_attr]
@@ -50,11 +75,12 @@ let bundle_map_ext
   (#[@@@erasable] fp2: Ghost.erased typ)
   ([@@@erasable] sp2: Ghost.erased (mg_spec t2 fp2 mb1.mb_spec_type true))
   ([@@@erasable] sq: squash (
-    impl_zero_copy_map_ext_precond (Ghost.reveal mb1.mb_typ) (mb1.mb_spec.mg_parser) (Ghost.reveal t2) sp2.mg_parser
+    impl_zero_copy_map_ext_precond (Ghost.reveal mb1.mb_typ) (mb1.mb_spec.mg_parser) (Ghost.reveal t2) sp2.mg_parser /\
+    impl_serialize_map_ext_precond (Ghost.reveal mb1.mb_spec) (Ghost.reveal sp2)
   ))
 : Tot (map_bundle vmatch)
 = match mb1 with
-  | Mkmap_bundle mb_typ mb_footprint mb_footprint_correct mb_spec_type mb_spec_type_eq mb_spec mb_impl_type mb_rel mb_parser ->
+  | Mkmap_bundle mb_typ mb_footprint mb_footprint_correct mb_spec_type mb_spec_type_eq mb_spec mb_impl_type mb_rel mb_parser mb_serializer ->
 {
   mb_typ = _;
   mb_footprint = _;
@@ -64,7 +90,8 @@ let bundle_map_ext
   mb_spec = sp2;
   mb_impl_type = _;
   mb_rel = _;
-  mb_parser = impl_zero_copy_map_ext #_ #_ #_ #_ #_ #_ #_ #mb_spec.mg_parser mb_parser #_ #_ #sp2.mg_size #sp2.mg_serializable sp2.mg_parser ()
+  mb_parser = impl_zero_copy_map_ext #_ #_ #_ #_ #_ #_ #_ #mb_spec.mg_parser mb_parser #_ #_ #sp2.mg_size #sp2.mg_serializable sp2.mg_parser ();
+  mb_serializer = impl_serialize_map_group_ext mb_serializer sp2 ();
 }
 
 inline_for_extraction noextract [@@noextract_to "krml"; bundle_get_impl_type_attr]
@@ -91,9 +118,9 @@ let bundle_map_choice
   ))
 : Tot (map_bundle vmatch)
 = match mb1 with
-  | Mkmap_bundle mb_typ1 mb_footprint1 mb_footprint_correct1 mb_spec_type1 mb_spec_type_eq1 mb_spec1 mb_impl_type1 mb_rel1 mb_parser1 ->
+  | Mkmap_bundle mb_typ1 mb_footprint1 mb_footprint_correct1 mb_spec_type1 mb_spec_type_eq1 mb_spec1 mb_impl_type1 mb_rel1 mb_parser1 mb_serializer1 ->
   match mb2 with
-  | Mkmap_bundle mb_typ2 mb_footprint2 mb_footprint_correct2 mb_spec_type2 mb_spec_type_eq2 mb_spec2 mb_impl_type2 mb_rel2 mb_parser2 ->
+  | Mkmap_bundle mb_typ2 mb_footprint2 mb_footprint_correct2 mb_spec_type2 mb_spec_type_eq2 mb_spec2 mb_impl_type2 mb_rel2 mb_parser2 mb_serializer2 ->
 {
   mb_typ = _;
   mb_footprint = _;
@@ -104,6 +131,7 @@ let bundle_map_choice
   mb_impl_type = _;
   mb_rel = _;
   mb_parser = impl_zero_copy_map_choice #_ #_ #_ #_ #_ #_ #_ #mb_spec1.mg_parser v1 mb_parser1 mb_parser2 ();
+  mb_serializer = impl_serialize_map_group_choice mb_serializer1 mb_serializer2 ();
 }
 
 inline_for_extraction noextract [@@noextract_to "krml"; bundle_get_impl_type_attr]
@@ -117,7 +145,7 @@ let bundle_map_zero_or_one
   ))
 : Tot (map_bundle vmatch)
 = match mb1 with
-  | Mkmap_bundle mb_typ mb_footprint mb_footprint_correct mb_spec_type mb_spec_type_eq mb_spec mb_impl_type mb_rel mb_parser ->
+  | Mkmap_bundle mb_typ mb_footprint mb_footprint_correct mb_spec_type mb_spec_type_eq mb_spec mb_impl_type mb_rel mb_parser mb_serializer ->
 {
   mb_typ = _;
   mb_footprint = _;
@@ -128,6 +156,7 @@ let bundle_map_zero_or_one
   mb_impl_type = _;
   mb_rel = _;
   mb_parser = impl_zero_copy_map_zero_or_one #_ #_ #_ #_ #_ #_ #_ #mb_spec.mg_parser v1 mb_parser ();
+  mb_serializer = impl_serialize_map_group_zero_or_one mb_serializer ();
 }
 
 inline_for_extraction noextract [@@noextract_to "krml"; bundle_get_impl_type_attr]
@@ -143,9 +172,9 @@ let bundle_map_concat
   ))
 : Tot (map_bundle vmatch)
 = match mb1 with
-  | Mkmap_bundle mb_typ1 mb_footprint1 mb_footprint_correct1 mb_spec_type1 mb_spec_type_eq1 mb_spec1 mb_impl_type1 mb_rel1 mb_parser1 ->
+  | Mkmap_bundle mb_typ1 mb_footprint1 mb_footprint_correct1 mb_spec_type1 mb_spec_type_eq1 mb_spec1 mb_impl_type1 mb_rel1 mb_parser1 mb_serializer1 ->
   match mb2 with
-  | Mkmap_bundle mb_typ2 mb_footprint2 mb_footprint_correct2 mb_spec_type2 mb_spec_type_eq2 mb_spec2 mb_impl_type2 mb_rel2 mb_parser2 ->
+  | Mkmap_bundle mb_typ2 mb_footprint2 mb_footprint_correct2 mb_spec_type2 mb_spec_type_eq2 mb_spec2 mb_impl_type2 mb_rel2 mb_parser2 mb_serializer2 ->
 {
   mb_typ = _;
   mb_footprint = _;
@@ -156,6 +185,7 @@ let bundle_map_concat
   mb_impl_type = _;
   mb_rel = _;
   mb_parser = impl_zero_copy_map_concat share gather mb_parser1 mb_parser2 ();
+  mb_serializer = impl_serialize_map_group_concat mb_serializer1 mb_serializer2 ();
 }
 
 inline_for_extraction noextract [@@noextract_to "krml"; bundle_get_impl_type_attr]
@@ -163,13 +193,15 @@ let bundle_map_match_item_for
   (#ty: Type0)
   (#vmatch: perm -> ty -> cbor -> slprop)
   (get: map_get_t vmatch)
+  (insert: cbor_det_serialize_map_insert_t)
+  (serialize: cbor_det_serialize_t vmatch)
   (#[@@@erasable] key: Ghost.erased cbor)
   (lkey: with_cbor_literal_t vmatch (Ghost.reveal key))
   ([@@@erasable] cut: Ghost.erased bool)
   (value: bundle vmatch)
 : Tot (map_bundle vmatch)
 = match value with
-  | Mkbundle b_typ b_spec_type b_spec_type_eq b_spec b_impl_type b_rel b_parser ->
+  | Mkbundle b_typ b_spec_type b_spec_type_eq b_spec b_impl_type b_rel b_parser b_serializer ->
 {
   mb_typ = _;
   mb_footprint = _;
@@ -180,6 +212,7 @@ let bundle_map_match_item_for
   mb_impl_type = _;
   mb_rel = _;
   mb_parser = impl_zero_copy_match_item_for get lkey cut b_parser;
+  mb_serializer = impl_serialize_match_item_for insert (CDDL.Pulse.Serialize.Misc.impl_serialize_literal serialize lkey) cut b_serializer;
 }
 
 module EqTest = CDDL.Spec.EqTest
@@ -190,9 +223,18 @@ let bundle_map_zero_or_more
   (#vmatch: perm -> ty -> cbor -> slprop)
   (#cbor_map_iterator_t: Type0)
   (#cbor_map_iterator_match: perm -> cbor_map_iterator_t -> list (cbor & cbor) -> slprop)
+  (#ty2: Type0) (#vmatch2: perm -> ty2 -> (cbor & cbor) -> slprop)
   (map_iterator_start: map_iterator_start_t vmatch cbor_map_iterator_match)
   (map_share: share_t cbor_map_iterator_match)
   (map_gather: gather_t cbor_map_iterator_match)
+  (map_is_empty: map_iterator_is_empty_t cbor_map_iterator_match)
+  (map_next: map_iterator_next_t vmatch2 cbor_map_iterator_match)
+  (map_entry_key: map_entry_key_t vmatch2 vmatch)
+  (map_entry_value: map_entry_value_t vmatch2 vmatch)
+  (map_entry_share: share_t vmatch2)
+  (map_entry_gather: gather_t vmatch2)
+  (parse: cbor_det_parse_t vmatch)
+  (insert: cbor_det_serialize_map_insert_t)
   (key: bundle vmatch) // MUST contain function pointers ONLY
   (va1: impl_typ vmatch key.b_typ) // MUST be a function pointer
   (#[@@@erasable] key_except: Ghost.erased typ)
@@ -201,9 +243,9 @@ let bundle_map_zero_or_more
   (va2: impl_typ vmatch value.b_typ) // MUST be a function pointer
 : Tot (map_bundle vmatch)
 = match key with
-  | Mkbundle b_typ1 b_spec_type1 b_spec_type_eq1 b_spec1 b_impl_type1 b_rel1 b_parser1 ->
+  | Mkbundle b_typ1 b_spec_type1 b_spec_type_eq1 b_spec1 b_impl_type1 b_rel1 b_parser1 b_serializer1 ->
   match value with
-  | Mkbundle b_typ2 b_spec_type2 b_spec_type_eq2 b_spec2 b_impl_type2 b_rel2 b_parser2 ->
+  | Mkbundle b_typ2 b_spec_type2 b_spec_type_eq2 b_spec2 b_impl_type2 b_rel2 b_parser2 b_serializer2 ->
 {
   mb_typ = _;
   mb_footprint = _;
@@ -213,5 +255,6 @@ let bundle_map_zero_or_more
   mb_spec = mg_zero_or_more_match_item b_spec1 key_except b_spec2;
   mb_impl_type = _;
   mb_rel = _;
-  mb_parser = impl_zero_copy_map_zero_or_more map_iterator_start map_share map_gather b_spec_type_eq1 b_spec1 va1 b_parser1 va_ex b_spec2 va2 b_parser2
+  mb_parser = impl_zero_copy_map_zero_or_more map_iterator_start map_share map_gather b_spec_type_eq1 b_spec1 va1 b_parser1 va_ex b_spec2 va2 b_parser2;
+  mb_serializer = impl_serialize_map_zero_or_more map_share map_gather map_is_empty map_next map_entry_key map_entry_value map_entry_share map_entry_gather parse insert #b_typ1 #b_spec_type1 b_spec_type_eq1 #b_spec1 #b_impl_type1 #b_rel1 b_serializer1 #key_except va_ex b_serializer2;
 }
