src/cddl/pulse/CDDL.Pulse.Bundle.ArrayGroup.fst
@@ -1,6 +1,7 @@
 module CDDL.Pulse.Bundle.ArrayGroup
 include CDDL.Pulse.Bundle.Base
 include CDDL.Pulse.Parse.ArrayGroup
+include CDDL.Pulse.Serialize.ArrayGroup
 open Pulse.Lib.Pervasives
 open CBOR.Spec.API.Type
 open CBOR.Pulse.API.Base
@@ -19,6 +20,7 @@ type array_bundle
   ab_impl_type: Type0;
   [@@@erasable] ab_rel: rel ab_impl_type ab_spec_type;
   ab_parser: impl_zero_copy_array_group cbor_array_iterator_match ab_spec.ag_parser ab_rel;
+  ab_serializer: impl_serialize_array_group ab_spec ab_rel;
 }
 
 inline_for_extraction noextract [@@noextract_to "krml"; bundle_get_impl_type_attr]
@@ -30,10 +32,10 @@ let get_array_bundle_impl_type
   (requires True)
   (ensures fun t -> t == b.ab_impl_type) // guard if the number of fields changes
 = match b with
-  | Mkarray_bundle _ _ _ _ ab_impl_type _ _ -> ab_impl_type
+  | Mkarray_bundle _ _ _ _ ab_impl_type _ _ _ -> ab_impl_type
 
 inline_for_extraction noextract [@@noextract_to "krml"; bundle_get_impl_type_attr]
-let array_bundle_set_parser
+let array_bundle_set_parser_and_serializer
   (#cbor_array_iterator_t: Type0)
   (#cbor_array_iterator_match: perm -> cbor_array_iterator_t -> list cbor -> slprop)
   ([@@@erasable] b: Ghost.erased (array_bundle cbor_array_iterator_match))
@@ -42,6 +44,9 @@ let array_bundle_set_parser
   (#[@@@erasable] t': Type)
   (p: t')
   ([@@@erasable] p_eq: squash (t' == impl_zero_copy_array_group cbor_array_iterator_match b.ab_spec.ag_parser b.ab_rel))
+  (#[@@@erasable] ts: Type)
+  (s: ts)
+  ([@@@erasable] s_eq: squash (ts == impl_serialize_array_group b.ab_spec b.ab_rel))
 : Tot (array_bundle cbor_array_iterator_match)
 = {
     ab_typ = b.ab_typ;
@@ -51,6 +56,7 @@ let array_bundle_set_parser
     ab_impl_type = t;
     ab_rel = coerce_eq () b.ab_rel;
     ab_parser = p;
+    ab_serializer = s;
   }
 
 inline_for_extraction noextract [@@noextract_to "krml"; bundle_get_impl_type_attr ]
@@ -60,10 +66,11 @@ let bundle_array
   (#cbor_array_iterator_t: Type)
   (#cbor_array_iterator_match: perm -> cbor_array_iterator_t -> list cbor -> slprop)
   (cbor_array_iterator_start: array_iterator_start_t vmatch cbor_array_iterator_match)
+  (cbor_serialize_array: cbor_det_serialize_array_t)
   (ab: array_bundle cbor_array_iterator_match)
 : Tot (bundle vmatch)
 = match ab with
-  | Mkarray_bundle ab_typ ab_spec_type ab_spec_type_eq ab_spec ab_impl_type ab_rel ab_parser ->
+  | Mkarray_bundle ab_typ ab_spec_type ab_spec_type_eq ab_spec ab_impl_type ab_rel ab_parser ab_serializer ->
 {
   b_typ = _;
   b_spec_type = _;
@@ -72,6 +79,7 @@ let bundle_array
   b_impl_type = ab_impl_type;
   b_rel = _;
   b_parser = impl_zero_copy_array cbor_array_iterator_start ab_parser;
+  b_serializer = impl_serialize_array cbor_serialize_array ab_serializer;
 }
 
 inline_for_extraction noextract [@@noextract_to "krml"; bundle_get_impl_type_attr]
@@ -82,13 +90,13 @@ let bundle_array_group_ext
   (#[@@@erasable] g2: Ghost.erased (array_group None))
   ([@@@erasable] sp2: Ghost.erased (ag_spec g2 ab.ab_spec_type true))
   ([@@@erasable] sq: squash (
-    array_group_included g2 ab.ab_typ /\
+    array_group_equiv g2 ab.ab_typ /\
     (forall (x: list cbor) . array_group_parser_spec_refinement g2 x ==> (
        (sp2.ag_parser x <: ab.ab_spec_type) == (ab.ab_spec.ag_parser x <: ab.ab_spec_type)
     ))
   ))
 = match ab with
-  | Mkarray_bundle ab_typ ab_spec_type ab_spec_type_eq ab_spec ab_impl_type ab_rel ab_parser ->
+  | Mkarray_bundle ab_typ ab_spec_type ab_spec_type_eq ab_spec ab_impl_type ab_rel ab_parser ab_serializer ->
 {
   ab_typ = _;
   ab_spec_type = _;
@@ -97,6 +105,7 @@ let bundle_array_group_ext
   ab_impl_type = ab_impl_type;
   ab_rel = _;
   ab_parser = impl_zero_copy_array_group_ext ab_parser #_ #sp2.ag_size #sp2.ag_serializable sp2.ag_parser ();
+  ab_serializer = impl_serialize_array_group_ext ab_serializer _ ();
 }
 
 inline_for_extraction noextract [@@noextract_to "krml"; bundle_get_impl_type_attr]
@@ -123,7 +132,7 @@ let bundle_array_group_item
   (b: bundle vmatch)
 : Tot (array_bundle cbor_array_iterator_match)
 = match b with
-  | Mkbundle b_typ b_spec_type b_spec_type_eq b_spec b_impl_type b_rel b_parser ->
+  | Mkbundle b_typ b_spec_type b_spec_type_eq b_spec b_impl_type b_rel b_parser b_serializer ->
 {
   ab_typ = _;
   ab_spec_type = _;
@@ -132,6 +141,7 @@ let bundle_array_group_item
   ab_impl_type = b_impl_type;
   ab_rel = _;
   ab_parser = impl_zero_copy_array_group_item cbor_array_iterator_next b_parser;
+  ab_serializer = impl_serialize_array_group_item b_serializer
 }
 
 inline_for_extraction noextract [@@noextract_to "krml"; bundle_get_impl_type_attr]
@@ -150,9 +160,9 @@ let bundle_array_group_concat
   ))
 : Tot (array_bundle cbor_array_iterator_match)
 = match b1 with
-  | Mkarray_bundle ab_typ1 ab_spec_type1 ab_spec_type_eq1 ab_spec1 ab_impl_type1 ab_rel1 ab_parser1 ->
+  | Mkarray_bundle ab_typ1 ab_spec_type1 ab_spec_type_eq1 ab_spec1 ab_impl_type1 ab_rel1 ab_parser1 ab_serializer1 ->
   match b2 with
-  | Mkarray_bundle ab_typ2 ab_spec_type2 ab_spec_type_eq2 ab_spec2 ab_impl_type2 ab_rel2 ab_parser2 ->
+  | Mkarray_bundle ab_typ2 ab_spec_type2 ab_spec_type_eq2 ab_spec2 ab_impl_type2 ab_rel2 ab_parser2 ab_serializer2 ->
 {
   ab_typ = _;
   ab_spec_type = _;
@@ -161,6 +171,7 @@ let bundle_array_group_concat
   ab_impl_type = (ab_impl_type1 & ab_impl_type2);
   ab_rel = _;
   ab_parser = impl_zero_copy_array_group_concat length share gather truncate ab_parser1 v1 ab_parser2 ();
+  ab_serializer = impl_serialize_array_group_concat ab_serializer1 ab_serializer2 ();
 }
 
 inline_for_extraction noextract [@@noextract_to "krml"; bundle_get_impl_type_attr]
@@ -175,9 +186,9 @@ let bundle_array_group_choice
   ))
 : Tot (array_bundle cbor_array_iterator_match)
 = match b1 with
-  | Mkarray_bundle ab_typ1 ab_spec_type1 ab_spec_type_eq1 ab_spec1 ab_impl_type1 ab_rel1 ab_parser1 ->
+  | Mkarray_bundle ab_typ1 ab_spec_type1 ab_spec_type_eq1 ab_spec1 ab_impl_type1 ab_rel1 ab_parser1 ab_serializer1 ->
   match b2 with
-  | Mkarray_bundle ab_typ2 ab_spec_type2 ab_spec_type_eq2 ab_spec2 ab_impl_type2 ab_rel2 ab_parser2 ->
+  | Mkarray_bundle ab_typ2 ab_spec_type2 ab_spec_type_eq2 ab_spec2 ab_impl_type2 ab_rel2 ab_parser2 ab_serializer2 ->
 {
   ab_typ = _;
   ab_spec_type = _;
@@ -186,6 +197,7 @@ let bundle_array_group_choice
   ab_impl_type = either ab_impl_type1 ab_impl_type2;
   ab_rel = _;
   ab_parser = impl_zero_copy_array_group_choice ab_parser1 v1 ab_parser2;
+  ab_serializer = impl_serialize_array_group_choice' ab_serializer1 ab_serializer2 ();
 }
 
 inline_for_extraction noextract [@@noextract_to "krml"; bundle_get_impl_type_attr]
@@ -199,7 +211,7 @@ let bundle_array_group_zero_or_one
   ))
 : Tot (array_bundle cbor_array_iterator_match)
 = match b1 with
-  | Mkarray_bundle ab_typ ab_spec_type ab_spec_type_eq ab_spec ab_impl_type ab_rel ab_parser ->
+  | Mkarray_bundle ab_typ ab_spec_type ab_spec_type_eq ab_spec ab_impl_type ab_rel ab_parser ab_serializer ->
 {  
   ab_typ = _;
   ab_spec_type = _;
@@ -208,14 +220,18 @@ let bundle_array_group_zero_or_one
   ab_impl_type = option ab_impl_type;
   ab_rel = _;
   ab_parser = impl_zero_copy_array_group_zero_or_one ab_parser v1;
+  ab_serializer = impl_serialize_array_group_zero_or_one ab_serializer ();
 }
 
 inline_for_extraction noextract [@@noextract_to "krml"; bundle_get_impl_type_attr]
 let bundle_array_group_zero_or_more
   (#cbor_array_iterator_t: Type)
   (#cbor_array_iterator_match: perm -> cbor_array_iterator_t -> list cbor -> slprop)
+  (is_empty: array_iterator_is_empty_t cbor_array_iterator_match)
+  (length: array_iterator_length_t cbor_array_iterator_match)
   (share: share_t cbor_array_iterator_match)
   (gather: gather_t cbor_array_iterator_match)
+  (truncate: array_iterator_truncate_t cbor_array_iterator_match)
   (b1: array_bundle cbor_array_iterator_match)
   (v1: impl_array_group cbor_array_iterator_match b1.ab_typ)
   ([@@@erasable] sq: squash (
@@ -224,7 +240,7 @@ let bundle_array_group_zero_or_more
   ))
 : array_bundle cbor_array_iterator_match
 = match b1 with
-  | Mkarray_bundle ab_typ ab_spec_type ab_spec_type_eq ab_spec ab_impl_type ab_rel ab_parser ->
+  | Mkarray_bundle ab_typ ab_spec_type ab_spec_type_eq ab_spec ab_impl_type ab_rel ab_parser ab_serializer ->
 {  
   ab_typ = _;
   ab_spec_type = _;
@@ -233,14 +249,18 @@ let bundle_array_group_zero_or_more
   ab_impl_type = _;
   ab_rel = _;
   ab_parser = impl_zero_copy_array_group_zero_or_more share gather #_ #_ #_ #_ #ab_spec.ag_parser v1 ab_parser ();
+  ab_serializer = impl_serialize_array_group_zero_or_more is_empty length share gather truncate ab_serializer ();
 }
 
 inline_for_extraction noextract [@@noextract_to "krml"; bundle_get_impl_type_attr]
 let bundle_array_group_one_or_more
   (#cbor_array_iterator_t: Type)
   (#cbor_array_iterator_match: perm -> cbor_array_iterator_t -> list cbor -> slprop)
+  (is_empty: array_iterator_is_empty_t cbor_array_iterator_match)
+  (length: array_iterator_length_t cbor_array_iterator_match)
   (share: share_t cbor_array_iterator_match)
   (gather: gather_t cbor_array_iterator_match)
+  (truncate: array_iterator_truncate_t cbor_array_iterator_match)
   (b1: array_bundle cbor_array_iterator_match)
   (v1: impl_array_group cbor_array_iterator_match b1.ab_typ)
   ([@@@erasable] sq: squash (
@@ -249,7 +269,7 @@ let bundle_array_group_one_or_more
   ))
 : array_bundle cbor_array_iterator_match
 = match b1 with
-  | Mkarray_bundle ab_typ ab_spec_type ab_spec_type_eq ab_spec ab_impl_type ab_rel ab_parser ->
+  | Mkarray_bundle ab_typ ab_spec_type ab_spec_type_eq ab_spec ab_impl_type ab_rel ab_parser ab_serializer ->
 {  
   ab_typ = _;
   ab_spec_type = _;
@@ -258,4 +278,5 @@ let bundle_array_group_one_or_more
   ab_impl_type = _;
   ab_rel = _;
   ab_parser = impl_zero_copy_array_group_one_or_more share gather #_ #_ #_ #_ #ab_spec.ag_parser v1 ab_parser ();
+  ab_serializer = impl_serialize_array_group_one_or_more is_empty length share gather truncate ab_serializer ();
 }
