src/cddl/pulse/CDDL.Pulse.Bundle.Base.fst
@@ -1,5 +1,6 @@
 module CDDL.Pulse.Bundle.Base
 include CDDL.Pulse.Parse.Base
+include CDDL.Pulse.Serialize.Base
 open Pulse.Lib.Pervasives
 open CBOR.Spec.API.Type
 module EqTest = CDDL.Spec.EqTest
@@ -17,6 +18,7 @@ type bundle
   b_impl_type: Type0;
   [@@@erasable] b_rel: rel b_impl_type b_spec_type;
   b_parser: impl_zero_copy_parse vmatch b_spec.parser b_rel;
+  b_serializer: impl_serialize b_spec b_rel;
 }
 
 irreducible let bundle_get_impl_type_attr : unit = ()
@@ -32,10 +34,10 @@ let get_bundle_impl_type
   (requires True)
   (ensures fun t -> t == b.b_impl_type) // guard if the number of fields changes
 = match b with
-  | Mkbundle _ _ _ _ b_impl_type _ _ -> b_impl_type
+  | Mkbundle _ _ _ _ b_impl_type _ _ _ -> b_impl_type
 
 inline_for_extraction noextract [@@noextract_to "krml"; bundle_get_impl_type_attr]
-let bundle_set_parser
+let bundle_set_parser_and_serializer
   (#cbor_t: Type)
   (#vmatch: perm -> cbor_t -> cbor -> slprop)
   ([@@@erasable] b: Ghost.erased (bundle vmatch))
@@ -44,6 +46,9 @@ let bundle_set_parser
   (#[@@@erasable] t': Type)
   (p: t')
   ([@@@erasable] p_eq: squash (t' == impl_zero_copy_parse vmatch b.b_spec.parser b.b_rel))
+  (#[@@@erasable] ts: Type)
+  (s: ts)
+  ([@@@erasable] s_eq: squash (ts == impl_serialize b.b_spec b.b_rel))
 : Tot (bundle vmatch)
 = {
     b_typ = b.b_typ;
@@ -52,25 +57,9 @@ let bundle_set_parser
     b_spec = b.b_spec;
     b_impl_type = t;
     b_rel = coerce_eq () b.b_rel;
-    b_parser = p
+    b_parser = p;
+    b_serializer = s;
   }
-
-inline_for_extraction noextract [@@noextract_to "krml"; bundle_get_impl_type_attr]
-let bundle_unit
-  (#cbor_t: Type)
-  (vmatch: perm -> cbor_t -> cbor -> slprop)
-  (#[@@@erasable] ty: Ghost.erased typ)
-  ([@@@erasable] sp: Ghost.erased (spec ty unit true))
-: bundle vmatch
-= {
-  b_typ = _;
-  b_spec_type = _;
-  b_spec_type_eq = EqTest.eqtype_eq _;
-  b_spec = sp;
-  b_impl_type = _;
-  b_rel = _;
-  b_parser = impl_zero_copy_unit _ _;
-}
 
 inline_for_extraction noextract [@@noextract_to "krml"; bundle_get_impl_type_attr]
 let bundle_always_false
@@ -87,6 +76,7 @@ let bundle_always_false
   b_impl_type = _;
   b_rel = _;
   b_parser = impl_zero_copy_always_false _ _;
+  b_serializer = impl_serialize_always_false _;
 }
 
 inline_for_extraction noextract [@@noextract_to "krml"; bundle_get_impl_type_attr]
@@ -97,11 +87,11 @@ let bundle_ext
   (#[@@@erasable] t': Ghost.erased typ)
   ([@@@erasable] sp': Ghost.erased (spec t' b.b_spec_type true))
   ([@@@erasable] sq: squash (
-    typ_included t' b.b_typ /\
+    typ_equiv t' b.b_typ /\
     (forall (x: cbor) . Ghost.reveal t' x ==> ((sp'.parser x <: b.b_spec_type) == b.b_spec.parser x))
   ))
 = match b with
-  | Mkbundle b_typ b_spec_type b_spec_type_eq b_spec b_impl_type b_rel b_parser ->
+  | Mkbundle b_typ b_spec_type b_spec_type_eq b_spec b_impl_type b_rel b_parser b_serializer ->
   {
   b_typ = t';
   b_spec_type = b_spec_type;
@@ -110,6 +100,7 @@ let bundle_ext
   b_impl_type = b_impl_type;
   b_rel = b_rel;
   b_parser = impl_zero_copy_ext b_parser #_ #sp'.serializable sp'.parser ();
+  b_serializer = impl_serialize_ext b_serializer _ ();
 }
 
 inline_for_extraction noextract [@@noextract_to "krml"; bundle_get_impl_type_attr]
@@ -135,9 +126,9 @@ let bundle_choice
     typ_disjoint b1.b_typ b2.b_typ
   ))
 = match b1 with
-  | Mkbundle b_typ1 b_spec_type1 b_spec_type_eq1 b_spec1 b_impl_type1 b_rel1 b_parser1 ->
+  | Mkbundle b_typ1 b_spec_type1 b_spec_type_eq1 b_spec1 b_impl_type1 b_rel1 b_parser1 b_serializer1 ->
   match b2 with
-  | Mkbundle b_typ2 b_spec_type2 b_spec_type_eq2 b_spec2 b_impl_type2 b_rel2 b_parser2 ->
+  | Mkbundle b_typ2 b_spec_type2 b_spec_type_eq2 b_spec2 b_impl_type2 b_rel2 b_parser2 b_serializer2 ->
   {
   b_typ = _;
   b_spec_type = _;
@@ -146,4 +137,5 @@ let bundle_choice
   b_impl_type = either b_impl_type1 b_impl_type2;
   b_rel = _;
   b_parser = impl_zero_copy_choice #_ #_ #_ #_ #_ #b_spec1.parser v1 b_parser1 b_parser2;
+  b_serializer = impl_serialize_choice b_serializer1 b_serializer2 ();
 }
