src/cddl/pulse/CDDL.Pulse.Bundle.Misc.fst
@@ -1,6 +1,7 @@
 module CDDL.Pulse.Bundle.Misc
 include CDDL.Pulse.Bundle.Base
 include CDDL.Pulse.Parse.Misc
+include CDDL.Pulse.Serialize.Misc
 open Pulse.Lib.Pervasives
 open CBOR.Spec.API.Type
 open CBOR.Pulse.API.Base
@@ -11,6 +12,9 @@ let bundle_uint
   (#cbor_t: Type)
   (#vmatch: perm -> cbor_t -> cbor -> slprop)
   (cbor_destr_int64: read_uint64_t vmatch)
+  (cbor_serialize: cbor_det_serialize_t vmatch)
+  (cbor_mk_int64: mk_int64_t vmatch)
+  (cbor_elim_int64: elim_int64_t vmatch)
 : bundle vmatch
 = {
   b_typ = _;
@@ -20,6 +24,7 @@ let bundle_uint
   b_impl_type = _;
   b_rel = _;
   b_parser = impl_copyful_pure_as_zero_copy (impl_copyful_uint cbor_destr_int64);
+  b_serializer = impl_serialize_uint cbor_serialize cbor_mk_int64 cbor_elim_int64;
 }
 
 inline_for_extraction noextract [@@noextract_to "krml"; bundle_get_impl_type_attr]
@@ -27,6 +32,9 @@ let bundle_nint
   (#cbor_t: Type)
   (#vmatch: perm -> cbor_t -> cbor -> slprop)
   (cbor_destr_int64: read_uint64_t vmatch)
+  (cbor_serialize: cbor_det_serialize_t vmatch)
+  (cbor_mk_int64: mk_int64_t vmatch)
+  (cbor_elim_int64: elim_int64_t vmatch)
 : bundle vmatch
 = {
   b_typ = _;
@@ -36,6 +44,7 @@ let bundle_nint
   b_impl_type = _;
   b_rel = _;
   b_parser = impl_copyful_pure_as_zero_copy (impl_copyful_nint cbor_destr_int64);
+  b_serializer = impl_serialize_nint cbor_serialize cbor_mk_int64 cbor_elim_int64;
 }
 
 module U64 = FStar.UInt64
@@ -45,7 +54,10 @@ let bundle_int_range_uint64
   (#cbor_t: Type)
   (#vmatch: perm -> cbor_t -> cbor -> slprop)
   (cbor_destr_int64: read_uint64_t vmatch)
-  (lo hi: Ghost.erased U64.t)
+  (cbor_serialize: cbor_det_serialize_t vmatch)
+  (cbor_mk_int64: mk_int64_t vmatch)
+  (cbor_elim_int64: elim_int64_t vmatch)
+  (lo hi: U64.t)
 : bundle vmatch
 = {
   b_typ = _;
@@ -55,6 +67,7 @@ let bundle_int_range_uint64
   b_impl_type = _;
   b_rel = _;
   b_parser = impl_copyful_pure_as_zero_copy (impl_copyful_int_range_uint64 cbor_destr_int64 lo hi);
+  b_serializer = impl_serialize_int_range_uint64 cbor_serialize cbor_mk_int64 cbor_elim_int64 lo hi;
 }
 
 module I64 = FStar.Int64
@@ -65,7 +78,10 @@ let bundle_int_range_int64
   (#vmatch: perm -> cbor_t -> cbor -> slprop)
   (cbor_get_major_type: get_major_type_t vmatch)
   (cbor_destr_int64: read_uint64_t vmatch)
-  (lo hi: Ghost.erased I64.t)
+  (cbor_serialize: cbor_det_serialize_t vmatch)
+  (cbor_mk_int64: mk_int64_t vmatch)
+  (cbor_elim_int64: elim_int64_t vmatch)
+  (lo hi: I64.t)
 : bundle vmatch
 = {
   b_typ = _;
@@ -75,6 +91,7 @@ let bundle_int_range_int64
   b_impl_type = _;
   b_rel = _;
   b_parser = impl_copyful_pure_as_zero_copy (impl_copyful_int_range_int64 cbor_get_major_type cbor_destr_int64 lo hi);
+  b_serializer = impl_serialize_int_range_int64 cbor_serialize cbor_mk_int64 cbor_elim_int64 lo hi;
 }
 
 inline_for_extraction noextract [@@noextract_to "krml"; bundle_get_impl_type_attr]
@@ -82,7 +99,10 @@ let bundle_int_range_neg_int64
   (#cbor_t: Type)
   (#vmatch: perm -> cbor_t -> cbor -> slprop)
   (cbor_destr_int64: read_uint64_t vmatch)
-  (lo hi: Ghost.erased U64.t)
+  (cbor_serialize: cbor_det_serialize_t vmatch)
+  (cbor_mk_int64: mk_int64_t vmatch)
+  (cbor_elim_int64: elim_int64_t vmatch)
+  (lo hi: U64.t)
 : bundle vmatch
 = {
   b_typ = _;
@@ -92,6 +112,7 @@ let bundle_int_range_neg_int64
   b_impl_type = _;
   b_rel = _;
   b_parser = impl_copyful_pure_as_zero_copy (impl_copyful_int_range_neg_int64 cbor_destr_int64 lo hi);
+  b_serializer = impl_serialize_int_range_neg_int64 cbor_serialize cbor_mk_int64 cbor_elim_int64 lo hi;
 }
 
 inline_for_extraction noextract [@@noextract_to "krml"; bundle_get_impl_type_attr]
@@ -99,6 +120,8 @@ let bundle_bytes
   (#cbor_t: Type)
   (#vmatch: perm -> cbor_t -> cbor -> slprop)
   (cbor_destr_string: get_string_t vmatch)
+  (cbor_serialize: cbor_det_serialize_t vmatch)
+  (cbor_mk_string: mk_string_t vmatch)
 : bundle vmatch
 = {
   b_typ = _;
@@ -108,6 +131,7 @@ let bundle_bytes
   b_impl_type = _;
   b_rel = _;
   b_parser = impl_zero_copy_bytes cbor_destr_string;
+  b_serializer = impl_serialize_bstr cbor_serialize cbor_mk_string false;
 }
 
 inline_for_extraction noextract [@@noextract_to "krml"; bundle_get_impl_type_attr]
@@ -115,6 +139,9 @@ let bundle_text
   (#cbor_t: Type)
   (#vmatch: perm -> cbor_t -> cbor -> slprop)
   (cbor_destr_string: get_string_t vmatch)
+  (impl_utf8_correct: impl_utf8_correct_t)
+  (cbor_serialize: cbor_det_serialize_t vmatch)
+  (cbor_mk_string: mk_string_t vmatch)
 : bundle vmatch
 = {
   b_typ = _;
@@ -124,6 +151,7 @@ let bundle_text
   b_impl_type = _;
   b_rel = _;
   b_parser = impl_zero_copy_text cbor_destr_string;
+  b_serializer = impl_serialize_tstr impl_utf8_correct cbor_serialize cbor_mk_string false;
 }
 
 inline_for_extraction noextract [@@noextract_to "krml"; bundle_get_impl_type_attr]
@@ -131,8 +159,11 @@ let bundle_str_size
   (#cbor_t: Type)
   (#vmatch: perm -> cbor_t -> cbor -> slprop)
   (cbor_destr_string: get_string_t vmatch)
-  (mt: Ghost.erased major_type_byte_string_or_text_string)
-  (lo hi: Ghost.erased U64.t)
+  (impl_utf8_correct: impl_utf8_correct_t)
+  (cbor_serialize: cbor_det_serialize_t vmatch)
+  (cbor_mk_string: mk_string_t vmatch)
+  (mt: major_type_byte_string_or_text_string)
+  (lo hi: U64.t)
 : bundle vmatch
 = {
   b_typ = _;
@@ -142,6 +173,7 @@ let bundle_str_size
   b_impl_type = _;
   b_rel = _;
   b_parser = impl_zero_copy_str_size cbor_destr_string mt lo hi;
+  b_serializer = impl_serialize_str_size impl_utf8_correct cbor_serialize cbor_mk_string false mt lo hi;
 }
 
 inline_for_extraction noextract [@@noextract_to "krml"; bundle_get_impl_type_attr]
@@ -149,6 +181,9 @@ let bundle_simple
   (#cbor_t: Type)
   (#vmatch: perm -> cbor_t -> cbor -> slprop)
   (cbor_destr_simple: read_simple_value_t vmatch)
+  (cbor_serialize: cbor_det_serialize_t vmatch)
+  (cbor_mk_simple: mk_simple_t vmatch)
+  (cbor_elim_simple: elim_simple_t vmatch)
 : bundle vmatch
 = {
   b_typ = _;
@@ -158,6 +193,7 @@ let bundle_simple
   b_impl_type = _;
   b_rel = _;
   b_parser = impl_copyful_pure_as_zero_copy (impl_copyful_simple cbor_destr_simple);
+  b_serializer = impl_serialize_simple cbor_serialize cbor_mk_simple cbor_elim_simple;
 }
 
 inline_for_extraction noextract [@@noextract_to "krml"; bundle_get_impl_type_attr]
@@ -165,6 +201,9 @@ let bundle_bool
   (#cbor_t: Type)
   (#vmatch: perm -> cbor_t -> cbor -> slprop)
   (cbor_destr_simple: read_simple_value_t vmatch)
+  (cbor_serialize: cbor_det_serialize_t vmatch)
+  (cbor_mk_simple: mk_simple_t vmatch)
+  (cbor_elim_simple: elim_simple_t vmatch)
 : bundle vmatch
 = {
   b_typ = _;
@@ -174,6 +213,7 @@ let bundle_bool
   b_impl_type = _;
   b_rel = _;
   b_parser = impl_copyful_pure_as_zero_copy (impl_copyful_bool cbor_destr_simple);
+  b_serializer = impl_serialize_bool cbor_serialize cbor_mk_simple cbor_elim_simple;
 }
 
 inline_for_extraction noextract [@@noextract_to "krml"; bundle_get_impl_type_attr]
@@ -181,11 +221,12 @@ let bundle_tagged_some
   (#cbor_t: Type)
   (#vmatch: perm -> cbor_t -> cbor -> slprop)
   (cbor_get_tagged_payload: get_tagged_payload_t vmatch)
-  (tag: Ghost.erased U64.t)
+  (cbor_serialize_tagged_tag: cbor_det_serialize_tag_t)
+  (tag: U64.t)
   (b: bundle vmatch)
 : bundle vmatch
 = match b with
-  | Mkbundle b_typ b_spec_type b_spec_type_eq b_spec b_impl_type b_rel b_parser ->
+  | Mkbundle b_typ b_spec_type b_spec_type_eq b_spec b_impl_type b_rel b_parser b_serializer ->
 {
   b_typ = _;
   b_spec_type = _;
@@ -194,6 +235,7 @@ let bundle_tagged_some
   b_impl_type = b_impl_type;
   b_rel = _;
   b_parser = impl_zero_copy_tagged_some cbor_get_tagged_payload tag b_parser;
+  b_serializer = impl_serialize_tagged_some cbor_serialize_tagged_tag tag b_serializer;
 }
 
 inline_for_extraction noextract [@@noextract_to "krml"; bundle_get_impl_type_attr]
@@ -202,10 +244,11 @@ let bundle_tagged_none
   (#vmatch: perm -> cbor_t -> cbor -> slprop)
   (cbor_get_tagged_tag: get_tagged_tag_t vmatch)
   (cbor_get_tagged_payload: get_tagged_payload_t vmatch)
+  (cbor_serialize_tagged_tag: cbor_det_serialize_tag_t)
   (b: bundle vmatch)
 : bundle vmatch
 = match b with
-  | Mkbundle b_typ b_spec_type b_spec_type_eq b_spec b_impl_type b_rel b_parser ->
+  | Mkbundle b_typ b_spec_type b_spec_type_eq b_spec b_impl_type b_rel b_parser b_serializer ->
 {
   b_typ = _;
   b_spec_type = _;
@@ -214,6 +257,7 @@ let bundle_tagged_none
   b_impl_type = (U64.t & b_impl_type);
   b_rel = _;
   b_parser = impl_zero_copy_tagged_none cbor_get_tagged_tag cbor_get_tagged_payload b_parser;
+  b_serializer = impl_serialize_tagged_none cbor_serialize_tagged_tag b_serializer;
 }
 
 inline_for_extraction noextract [@@noextract_to "krml"; bundle_get_impl_type_attr]
@@ -223,10 +267,11 @@ let bundle_det_cbor
   (#vmatch': perm -> cbor_t -> cbor -> slprop)
   (cbor_destr_string: get_string_t vmatch)
   (cbor_det_parse: cbor_det_parse_t vmatch')
+  (cbor_serialize_string: cbor_det_serialize_string_t)
   (b: bundle vmatch')
 : bundle vmatch
 = match b with
-  | Mkbundle b_typ b_spec_type b_spec_type_eq b_spec b_impl_type b_rel b_parser ->
+  | Mkbundle b_typ b_spec_type b_spec_type_eq b_spec b_impl_type b_rel b_parser b_serializer ->
 {
   b_typ = _;
   b_spec_type = _;
@@ -235,12 +280,14 @@ let bundle_det_cbor
   b_impl_type = b_impl_type;
   b_rel = _;
   b_parser = impl_zero_copy_det_cbor cbor_destr_string cbor_det_parse b_spec b_parser;
+  b_serializer = impl_serialize_bstr_cbor_det cbor_serialize_string b_serializer;
 }
 
 inline_for_extraction noextract [@@noextract_to "krml"; bundle_get_impl_type_attr]
 let bundle_any
   (#cbor_t: Type)
   (vmatch: perm -> cbor_t -> cbor -> slprop)
+  (cbor_serialize: cbor_det_serialize_t vmatch)
 : bundle vmatch
 = {
   b_typ = _;
@@ -250,4 +297,24 @@ let bundle_any
   b_impl_type = _;
   b_rel = _;
   b_parser = impl_zero_copy_any vmatch;
+  b_serializer = impl_serialize_any cbor_serialize;
+}
+
+inline_for_extraction noextract [@@noextract_to "krml"; bundle_get_impl_type_attr]
+let bundle_literal
+  (#cbor_t: Type)
+  (vmatch: perm -> cbor_t -> cbor -> slprop)
+  (cbor_serialize: cbor_det_serialize_t vmatch)
+  (# [@@@erasable] l: Ghost.erased cbor)
+  (w: with_cbor_literal_t vmatch l)
+: bundle vmatch
+= {
+  b_typ = _;
+  b_spec_type = _;
+  b_spec_type_eq = EqTest.eqtype_eq _;
+  b_spec = spec_literal l;
+  b_impl_type = _;
+  b_rel = _;
+  b_parser = impl_zero_copy_unit vmatch _;
+  b_serializer = impl_serialize_literal cbor_serialize w;
 }
