src/cddl/pulse/CDDL.Pulse.Serialize.MapGroup.fsti
@@ -12,6 +12,7 @@ module SZ = FStar.SizeT
 module Cbor = CBOR.Spec.API.Format
 module U64 = FStar.UInt64
 module Iterator = CDDL.Pulse.Iterator.Base
+module EqTest = CDDL.Spec.EqTest
 
 let impl_serialize_map_group_pre
   (count: U64.t)
@@ -93,3 +94,173 @@ val impl_serialize_map
     (i: impl_serialize_map_group s r)
     (sq: squash (map_group_footprint t fp))
 : impl_serialize #_ #_ #_ (spec_map_group s) #_ r
+
+inline_for_extraction noextract [@@noextract_to "krml"]
+val impl_serialize_map_group_ext
+    (#[@@@erasable]t: Ghost.erased (det_map_group))
+    (# [@@@erasable] fp: Ghost.erased typ)
+    (#[@@@erasable]tgt: Type0)
+    (#[@@@erasable] inj: Ghost.erased bool)
+    (#[@@@erasable]ps: Ghost.erased (mg_spec t fp tgt inj))
+    (#impl_tgt: Type0)
+    (#[@@@erasable]r: rel impl_tgt tgt)
+    (i: impl_serialize_map_group ps r)
+    (#[@@@erasable]t': Ghost.erased (det_map_group))
+    (# [@@@erasable] fp': Ghost.erased typ)
+    (#[@@@erasable] inj': Ghost.erased bool)
+    ([@@@erasable]ps': Ghost.erased (mg_spec t' fp' tgt inj'))
+    ([@@@erasable]sq: squash (
+      t' == t /\
+      (forall (x: tgt) . (Ghost.reveal ps').mg_serializable x <==> (Ghost.reveal ps).mg_serializable x) /\
+      (forall (x: tgt) . (Ghost.reveal ps').mg_serializable x ==> (
+        (Ghost.reveal ps).mg_serializable x /\
+        (Ghost.reveal ps').mg_serializer x `cbor_map_equal` (Ghost.reveal ps).mg_serializer x
+      )) /\
+      (forall (x: tgt) . (Ghost.reveal ps').mg_size x == (Ghost.reveal ps).mg_size x)
+    ))
+: impl_serialize_map_group #(Ghost.reveal t') #(Ghost.reveal fp') #tgt #inj' (Ghost.reveal ps') #impl_tgt r
+
+inline_for_extraction noextract [@@noextract_to "krml"]
+val impl_serialize_map_group_ext'
+    (#[@@@erasable]t: Ghost.erased (det_map_group))
+    (# [@@@erasable] fp: Ghost.erased typ)
+    (#[@@@erasable]tgt: Type0)
+    (#[@@@erasable] inj: Ghost.erased bool)
+    (#[@@@erasable]ps: Ghost.erased (mg_spec t fp tgt inj))
+    (#impl_tgt: Type0)
+    (#[@@@erasable]r: rel impl_tgt tgt)
+    (i: impl_serialize_map_group ps r)
+    ([@@@erasable] fp': Ghost.erased typ)
+    (sq: squash (
+      typ_equiv fp fp'
+    ))
+: impl_serialize_map_group #(Ghost.reveal t) #(Ghost.reveal fp') #tgt #inj (mg_spec_ext ps fp' ps.mg_size ps.mg_serializable) #impl_tgt r
+
+inline_for_extraction noextract [@@noextract_to "krml"]
+val impl_serialize_map_group_choice
+    (#[@@@erasable]t1: Ghost.erased det_map_group)
+    (#[@@@erasable]tgt1: Type0)
+    (#[@@@erasable] fp1: Ghost.erased typ)
+    (#[@@@erasable] inj1: Ghost.erased bool)
+    (#[@@@erasable]ps1: Ghost.erased (mg_spec t1 fp1 tgt1 inj1))
+    (#impl_tgt1: Type0)
+    (#[@@@erasable]r1: rel impl_tgt1 tgt1)
+    (i1: impl_serialize_map_group ps1 r1)
+    (#[@@@erasable]t2: Ghost.erased det_map_group)
+    (#[@@@erasable]tgt2: Type0)
+    (#[@@@erasable] fp2: Ghost.erased typ)
+    (#[@@@erasable] inj2: Ghost.erased bool)
+    (#[@@@erasable]ps2: Ghost.erased (mg_spec t2 fp2 tgt2 inj2))
+    (#impl_tgt2: Type0)
+    (#[@@@erasable]r2: rel impl_tgt2 tgt2)
+    (i2: impl_serialize_map_group ps2 r2)
+    (sq: squash (
+      map_group_footprint t1 fp1 /\
+      map_group_footprint t2 fp2 /\
+      map_group_choice_compatible t1 t2
+    ))
+: impl_serialize_map_group #_ #_ #_ #_ (mg_spec_choice ps1 ps2) #_ (rel_either r1 r2)
+
+inline_for_extraction noextract [@@noextract_to "krml"]
+val impl_serialize_map_group_zero_or_one
+    (#[@@@erasable]t1: Ghost.erased det_map_group)
+    (#[@@@erasable]tgt1: Type0)
+    (#[@@@erasable] fp1: Ghost.erased typ)
+    (#[@@@erasable] inj1: Ghost.erased bool)
+    (#[@@@erasable]ps1: Ghost.erased (mg_spec t1 fp1 tgt1 inj1))
+    (#impl_tgt1: Type0)
+    (#[@@@erasable]r1: rel impl_tgt1 tgt1)
+    (i1: impl_serialize_map_group ps1 r1)
+    (sq: squash (
+      map_group_footprint t1 fp1 /\
+      MapGroupFail? (apply_map_group_det t1 cbor_map_empty)
+    ))
+: impl_serialize_map_group #_ #_ #_ #_ (mg_spec_zero_or_one ps1) #_ (rel_option r1)
+
+inline_for_extraction noextract [@@noextract_to "krml"]
+val impl_serialize_map_group_either_left
+    (#[@@@erasable]t1: Ghost.erased det_map_group)
+    (#[@@@erasable]tgt1: Type0)
+    (#[@@@erasable] fp1: Ghost.erased typ)
+    (#[@@@erasable] inj1: Ghost.erased bool)
+    (#[@@@erasable]ps1: Ghost.erased (mg_spec t1 fp1 tgt1 inj1))
+    (#impl_tgt1: Type0)
+    (#[@@@erasable]r1: rel impl_tgt1 tgt1)
+    (i1: impl_serialize_map_group ps1 r1)
+    (#impl_tgt2: Type0)
+    (#[@@@erasable]r2: rel impl_tgt2 tgt1)
+    (i2: impl_serialize_map_group ps1 r2)
+: impl_serialize_map_group #_ #_ #_ #_ ps1 #_ (rel_either_left r1 r2)
+
+inline_for_extraction noextract [@@noextract_to "krml"]
+val impl_serialize_map_group_concat
+    (#[@@@erasable]t1: Ghost.erased det_map_group)
+    (#[@@@erasable]tgt1: Type0)
+    (#[@@@erasable] fp1: Ghost.erased typ)
+    (#[@@@erasable] inj1: Ghost.erased bool)
+    (#[@@@erasable]ps1: Ghost.erased (mg_spec t1 fp1 tgt1 inj1))
+    (#impl_tgt1: Type0)
+    (#[@@@erasable]r1: rel impl_tgt1 tgt1)
+    (i1: impl_serialize_map_group ps1 r1)
+    (#[@@@erasable]t2: Ghost.erased det_map_group)
+    (#[@@@erasable]tgt2: Type0)
+    (#[@@@erasable] fp2: Ghost.erased typ)
+    (#[@@@erasable] inj2: Ghost.erased bool)
+    (#[@@@erasable]ps2: Ghost.erased (mg_spec t2 fp2 tgt2 inj2))
+    (#impl_tgt2: Type0)
+    (#[@@@erasable]r2: rel impl_tgt2 tgt2)
+    (i2: impl_serialize_map_group ps2 r2)
+    (sq: squash (
+      map_group_footprint t1 fp1 /\
+      map_group_footprint t2 fp2 /\
+      typ_disjoint fp1 fp2
+    ))
+: impl_serialize_map_group #_ #_ #_ #_ (mg_spec_concat ps1 ps2) #_ (rel_pair r1 r2)
+
+inline_for_extraction
+val impl_serialize_match_item_for
+  (insert: cbor_det_serialize_map_insert_t)
+  (#[@@@erasable]key: Ghost.erased cbor)
+  (ik: impl_serialize (spec_literal key) rel_unit)
+  ([@@@erasable]cut: Ghost.erased bool)
+  (#[@@@erasable]value: Ghost.erased typ)
+  (#[@@@erasable]tvalue: Type0)
+  (#[@@@erasable]vinj: Ghost.erased bool)
+  (#[@@@erasable]pvalue: Ghost.erased (spec value tvalue vinj))
+  (#iv: Type0)
+  (#[@@@erasable]r: rel iv tvalue)
+  (ivalue: impl_serialize pvalue r)
+: impl_serialize_map_group #_ #_ #_ #_ (mg_spec_match_item_for cut key pvalue) #_ r
+
+inline_for_extraction noextract [@@noextract_to "krml"]
+val impl_serialize_map_zero_or_more
+  (#ty: Type0) (#vmatch: perm -> ty -> cbor -> slprop) (#cbor_map_iterator_t: Type0) (#cbor_map_iterator_match: perm -> cbor_map_iterator_t -> list (cbor & cbor) -> slprop)
+  (#ty2: Type0) (#vmatch2: perm -> ty2 -> (cbor & cbor) -> slprop)
+  (map_share: share_t cbor_map_iterator_match)
+  (map_gather: gather_t cbor_map_iterator_match)
+  (map_is_empty: map_iterator_is_empty_t cbor_map_iterator_match)
+  (map_next: map_iterator_next_t vmatch2 cbor_map_iterator_match)
+  (map_entry_key: map_entry_key_t vmatch2 vmatch)
+  (map_entry_value: map_entry_value_t vmatch2 vmatch)
+  (map_entry_share: share_t vmatch2)
+  (map_entry_gather: gather_t vmatch2)
+  (#ty': Type0) (#vmatch': perm -> ty' -> cbor -> slprop)
+  (parse: cbor_det_parse_t vmatch')
+  (insert: cbor_det_serialize_map_insert_t)
+    (#[@@@erasable]key: Ghost.erased typ)
+    (#[@@@erasable]tkey: Type0)
+    ([@@@erasable]key_eq: Ghost.erased (EqTest.eq_test tkey))
+    (#[@@@erasable]sp1: Ghost.erased (spec key tkey true))
+    (#ikey: Type0)
+    (#[@@@erasable]r1: rel ikey tkey)
+    (pa1: impl_serialize sp1 r1)
+    (#[@@@erasable]key_except: Ghost.erased typ)
+    (va_ex: impl_typ vmatch' key_except)
+    (#[@@@erasable]value: Ghost.erased typ)
+    (#[@@@erasable]tvalue: Type0)
+    (#[@@@erasable]inj: Ghost.erased bool)
+    (#[@@@erasable]sp2: Ghost.erased (spec value tvalue inj))
+    (#ivalue: Type0)
+    (#[@@@erasable]r2: rel ivalue tvalue)
+    (pa2: impl_serialize sp2 r2)
+: impl_serialize_map_group #(map_group_zero_or_more_match_item key key_except value) #_ #_ #_ (mg_zero_or_more_match_item sp1 key_except sp2) #_ (rel_either_left (rel_slice_of_table key_eq r1 r2) (rel_map_iterator vmatch cbor_map_iterator_match ikey ivalue (Iterator.mk_spec r1) (Iterator.mk_spec r2)))
